Updated

art/sqrt.v
@@ -1,6 +1,6 @@
 
 Require Import ZArith. 
-Require Import CoqArt.chap15 . 
+Require Export CoqArt.chap15 . 
 Open Scope Z_scope. 
 
 
@@ -114,36 +114,6 @@ Check Z.to_nat.
 
 Print div.  
 
-(* ex. 15.11 *) 
-Require Import Wellfounded. 
-Search (well_founded lt). 
-
-Open Scope nat. 
-
-Definition sqrt_type (n:nat)        := {s & {r | n = s*s+r /\ n < (S s)*(S s) } } .  
-(*
-    Definition sqrt_type' (n s:nat)     :=      {r | n = s*s+r /\ n < (s+1)*(s+1) }   .  
-    Definition sqrt_type'' (n s r:nat)  :=           n = s*s+r /\ n < (s+1)*(s+1)     .  
- *)
-Definition sqrt_WF : 
-  forall x, (forall y, y < x -> sqrt_type y) -> sqrt_type x. 
-Proof. 
-  intros. destruct x. 
-  - intros. exists 0, 0. now compute. 
-  - destruct (div (S x) 4) as [q [r0 [H1 H2]]]; auto with zarith. 
-    + destruct (H q) as [s' [r' [H1' H2']]]; auto with zarith.  
-      * { case (le_lt_dec (S(4*s')) (4*r'+r0)).   
-        - intros. exists (S(2*s')), (4*r'+r0-4*s'-1). auto with zarith.            
-        - intros. exists (2*s'   ), (4*r'+r0       ). auto with zarith. }
-Qed. 
-
-Check le_lt_dec. 
-
-Definition sqrt : forall n:nat, {s & { r | n = s*s+r /\ n < (S s)*(S s) }} :=
-  well_founded_induction lt_wf sqrt_type sqrt_WF. 
-
-Eval compute in  match sqrt 10 with 
-  existT _ s _ => s end. 
   
 Eval compute in match div 1000 13 _ with 
     existT _ s _ => s end. 
